A spec for slice.for_range; allows for loop unfolding in proof

new/golang/defn/slice.v
@@ -51,8 +51,8 @@ Definition full_slice t : val :=
 Definition for_range t : val :=
   λ: "s" "body",
   let: "i" := ref_ty uint64T (zero_val uint64T) in
-  for: ("i" < len "s") ; Skip :=
-    "body" "i" (![t] (elem_ref t "s"))
+  for: (λ: <>, ![uint64T] "i" < len "s") ; (λ: <>, "i" <-[uint64T] (![uint64T] "i") + #1) :=
+    (λ: <>, "body" (![uint64T] "i") (![t] (elem_ref t "s" (![uint64T] "i"))))
 .
 
 Definition copy t : val :=
