new/proof/grove_ffi.v
@@ -121,7 +121,7 @@ Section grove.
   Proof.
     iIntros "!#" (Φ) "Hs HΦ". wp_rec. 
     destruct s. wp_pures.
-    iDestruct (own_slice_sz with "Hs") as "%Hlen".
+    iDestruct (own_slice_len with "Hs") as "%Hlen".
     iDestruct (own_slice_wf with "Hs") as "%Hwf".
     rewrite difference_empty_L.
     iMod "HΦ" as (ms) "[Hc HΦ]".
@@ -224,7 +224,7 @@ Section grove.
     iCache with "HΦ Hf". { iApply "HΦ". by iLeft. }
     (* Urgh so much manual work just calling a WP lemma... *)
     wpc_pures.
-    iDestruct (own_slice_sz with "Hs") as "%Hlen".
+    iDestruct (own_slice_len with "Hs") as "%Hlen".
     iDestruct (own_slice_wf with "Hs") as "%Hwf".
     wpc_bind (ExternalOp _ _).
     wpc_bind (slice.ptr _). wpc_frame. wp_pures. iModIntro. iNamed 1.
@@ -264,7 +264,7 @@ Section grove.
     iCache with "HΦ Hf". { iApply "HΦ". by iLeft. }
     (* Urgh so much manual work just calling a WP lemma... *)
     wpc_pures.
-    iDestruct (own_slice_sz with "Hs") as "%Hlen".
+    iDestruct (own_slice_len with "Hs") as "%Hlen".
     iDestruct (own_slice_wf with "Hs") as "%Hwf".
     wpc_bind (slice.ptr _). wpc_frame. wp_pures. iModIntro. iNamed 1.
     wpc_bind (slice.len _). wpc_frame. wp_pures. iModIntro. iNamed 1.
